Various merge cleanup fixes.

src/tls/Format.UncompressedPointRepresentation.fst
@@ -7,7 +7,11 @@ module U8 = FStar.UInt8
 module U32 = FStar.UInt32
 module LP = LowParse.SLow
 
+unfold type is_injective (#a:Type) (#b:Type) (f:a -> b) 
+  = forall x y . f x == f y ==> x == y
 
+unfold type is_injective_2 (#a:Type) (#b:Type) (f:a -> b) (x:a) (y:a)
+  = f x == f y ==> x == y
 (* Types *)
 
 (*
@@ -20,65 +24,84 @@ module LP = LowParse.SLow
     } UncompressedPointRepresentation;
 *)
 
-type uncompressedPointRepresentation (coordinate_length:nat) = {
+type lbytes32 (l:U32.t) = B.lbytes (UInt32.v l)
+
+type uncompressedPointRepresentation (coordinate_length:U32.t) = {
     legacy_form : l:B.byte{l = 4uy};
-    x           : B.lbytes coordinate_length;
-    y           : B.lbytes coordinate_length
+    x           : b:lbytes32 coordinate_length;
+    y           : b:lbytes32 coordinate_length;
 }
 
 private 
-type lbytes_pair (coordinate_length:nat) = (B.lbytes coordinate_length * B.lbytes coordinate_length)
+type lbytes_pair (coordinate_length:U32.t) = (lbytes32 coordinate_length) * (lbytes32 coordinate_length)
 
 
 (* Parsers *)
 
 private
-let lbytes_pair_parser_kind (coordinate_length:nat)
+let lbytes_pair_parser_kind (coordinate_length:U32.t)
   : LP.parser_kind
-  = LP.and_then_kind 
-      (LP.total_constant_size_parser_kind coordinate_length) 
-      (LP.total_constant_size_parser_kind coordinate_length)
+  = let l = (UInt32.v coordinate_length) in
+    LP.and_then_kind 
+      (LP.total_constant_size_parser_kind l)
+      (LP.total_constant_size_parser_kind l)
 
-let lbytes_pair_parser (coordinate_length:nat)
+let lbytes_pair_parser (coordinate_length:U32.t)
   : LP.parser (lbytes_pair_parser_kind coordinate_length) (lbytes_pair coordinate_length)
-  = LP.nondep_then
-      (LP.parse_flbytes coordinate_length)
-      (LP.parse_flbytes coordinate_length)
+  = let l = UInt32.v coordinate_length in
+    LP.nondep_then
+      (LP.parse_flbytes l)
+      (LP.parse_flbytes l)
 
+#reset-options "--using_facts_from '* -LowParse -FStar.Reflection -FStar.Tactics' --max_fuel 16 --initial_fuel 16 --max_ifuel 16 --initial_ifuel 16"
 private
 inline_for_extraction
-let lbytes_pair_parser32 (coordinate_length:nat)
+let lbytes_pair_parser32 (coordinate_length:U32.t)
   : LP.parser32 (lbytes_pair_parser coordinate_length) 
-  = LP.parse32_nondep_then
-      (LP.parse32_flbytes coordinate_length (U32.uint_to_t coordinate_length))
-      (LP.parse32_flbytes coordinate_length (U32.uint_to_t coordinate_length))
+  = let l = UInt32.v coordinate_length in
+    LP.parse32_nondep_then
+      (LP.parse32_flbytes l coordinate_length)
+      (LP.parse32_flbytes l coordinate_length)
+#reset-options
 
-
-let uncompressedPointRepresentation_parser_kind (coordinate_length:nat) 
+let uncompressedPointRepresentation_parser_kind (coordinate_length:U32.t) 
   = LP.and_then_kind
       constantByte_parser_kind
       (lbytes_pair_parser_kind coordinate_length)
 
 private
 inline_for_extraction
-let ucp_of_uv (#n:nat) (p:(B.lbytes n) * (B.lbytes n))
+let ucp_of_uv (#n:U32.t) (p:(lbytes32 n) * (lbytes32 n))
   : uncompressedPointRepresentation n
   = { legacy_form = 4uy; x = (fst p); y = (snd p) }
 
 private
 inline_for_extraction
-let uv_of_ucp (#n:nat) (x:uncompressedPointRepresentation n)
-  : Tot (B.byte * (B.lbytes n * B.lbytes n))
-  = (4uy, (x.x, x.y))
+let uv_of_ucp (#n:U32.t) (x:uncompressedPointRepresentation n)
+  : Tot (lbytes32 n * lbytes32 n)
+  = (x.x, x.y)
 
-let uncompressedPointRepresentation_parser (coordinate_length:nat)
+#reset-options "--using_facts_from '* -LowParse -FStar.Reflection -FStar.Tactics' --max_fuel 16 --initial_fuel 16 --max_ifuel 16 --initial_ifuel 16"
+let lemma_ucp_of_uv_is_injective #l
+  : Lemma (is_injective (ucp_of_uv #l))
+  = ()
+#reset-options
+
+#reset-options "--using_facts_from '* -LowParse -FStar.Reflection -FStar.Tactics' --max_fuel 16 --initial_fuel 16 --max_ifuel 16 --initial_ifuel 16 --z3rlimit 10"
+let lemma_ucp_of_uv_of_ucp #l 
+  : Lemma (forall x . ucp_of_uv #l (uv_of_ucp #l x) == x)
+  = lemma_ucp_of_uv_is_injective #l
+#reset-options
+
+
+let uncompressedPointRepresentation_parser (coordinate_length:U32.t)
   : LP.parser (uncompressedPointRepresentation_parser_kind coordinate_length) (uncompressedPointRepresentation coordinate_length) 
   = LP.parse_synth
       (LP.nondep_then (constantByte_parser 4uy) (lbytes_pair_parser coordinate_length))
       (fun (c, uv) -> ucp_of_uv uv)
 
 inline_for_extraction
-let uncompressedPointRepresentation_parser32 (coordinate_length:nat)
+let uncompressedPointRepresentation_parser32 (coordinate_length:U32.t)
   : LP.parser32 (uncompressedPointRepresentation_parser coordinate_length)
   = LP.parse32_synth
       (LP.nondep_then (constantByte_parser 4uy) (lbytes_pair_parser coordinate_length))
@@ -87,26 +110,35 @@ let uncompressedPointRepresentation_parser32 (coordinate_length:nat)
       (LP.parse32_nondep_then (constantByte_parser32 4uy) (lbytes_pair_parser32 coordinate_length))
       ()
 
+
 (* Serializers *)
 
+#reset-options "--using_facts_from '* -LowParse -FStar.Reflection -FStar.Tactics' --max_fuel 16 --initial_fuel 16 --max_ifuel 16 --initial_ifuel 16 --z3rlimit 10"
 private
-let lbytes_pair_serializer (coordinate_length:nat)
+let lbytes_pair_serializer (coordinate_length:U32.t)
   : LP.serializer (lbytes_pair_parser coordinate_length) 
-  = let p = LP.parse_flbytes coordinate_length in
-    let s = LP.serialize_flbytes coordinate_length in
+  = let l = U32.v coordinate_length in
+    // lemma_ucp_of_uv_is_injective #coordinate_length;
+    // lemma_ucp_of_uv_of_ucp #coordinate_length;
+    let p = LP.parse_flbytes l in
+    let s = LP.serialize_flbytes l in
+    assert (LP.Mkparser_kind'?.parser_kind_subkind (LP.get_parser_kind p) == Some LP.ParserStrong);
     LP.serialize_nondep_then p s () p s
 
 private
 inline_for_extraction
-let lbytes_pair_serializer32 (coordinate_length:nat)
+let lbytes_pair_serializer32 (coordinate_length:U32.t)
   : LP.serializer32 (lbytes_pair_serializer coordinate_length) 
-  = LP.serialize32_nondep_then
-      (LP.serialize32_flbytes coordinate_length) ()
-      (LP.serialize32_flbytes coordinate_length) ()
+  = let l = U32.v coordinate_length in
+    LP.serialize32_nondep_then
+      (LP.serialize32_flbytes l) ()
+      (LP.serialize32_flbytes l) ()
 
-let uncompressedPointRepresentation_serializer (coordinate_length:nat) 
+
+let uncompressedPointRepresentation_serializer (coordinate_length:U32.t) 
   : LP.serializer (uncompressedPointRepresentation_parser coordinate_length)
-  = LP.serialize_synth
+  = let l = U32.v coordinate_length in
+    LP.serialize_synth
       (LP.nondep_then (constantByte_parser 4uy) (lbytes_pair_parser coordinate_length))
       (fun (c, uv) -> ucp_of_uv uv)
       (LP.serialize_nondep_then 
@@ -119,20 +151,16 @@ let uncompressedPointRepresentation_serializer (coordinate_length:nat)
       ()
 
 inline_for_extraction
-let uncompressedPointRepresentation_serializer32 (coordinate_length:nat) 
+let uncompressedPointRepresentation_serializer32 (coordinate_length:U32.t) 
   : LP.serializer32 (uncompressedPointRepresentation_serializer coordinate_length)
   = LP.serialize32_synth
-      (LP.nondep_then (constantByte_parser 4uy) (lbytes_pair_parser coordinate_length))
+      _
       (fun (c, uv) -> ucp_of_uv uv)
-      (LP.serialize_nondep_then 
-        (constantByte_parser 4uy)
-        (constantByte_serializer 4uy) 
-        ()
-        (lbytes_pair_parser coordinate_length)
-        (lbytes_pair_serializer coordinate_length))
+      _
       (LP.serialize32_nondep_then 
         (constantByte_serializer32 4uy) ()
         (lbytes_pair_serializer32 coordinate_length) ())
-      uv_of_ucp
-      uv_of_ucp
+      (fun x -> 4uy, uv_of_ucp x)
+      (fun x -> 4uy, uv_of_ucp x)
       ()
+#reset-options
